proof/theories/Ip6_Nat.v
@@ -140,7 +140,7 @@ Definition pkt6 : packet :=
      pkt_fibkey := fun _ => []; pkt_numgen := fun _ => []; pkt_osf := [];
      pkt_tunnel := fun _ => []; pkt_symhash := fun _ _ => [];
      pkt_xfrm := fun _ _ _ => []; pkt_ctdir := fun _ _ => [];
-     pkt_inner := fun _ _ _ _ => []; pkt_have_l2 := true; pkt_have_l4 := false; pkt_fragoff := 0; pkt_flow := []; pkt_untracked := false; pkt_ctdir_orig := true |}.
+     pkt_inner := fun _ _ _ _ => []; pkt_have_l2 := true; pkt_have_l4 := false; pkt_fragoff := 0; pkt_flow := []; pkt_untracked := false; pkt_ctdir_orig := true; pkt_ct_present := true |}.
 
 Theorem ip6_dnat_dest_is_target :
   field_value FIp6Daddr (apply_nat Hprerouting ip6_dnat_rule pkt6) = tgt6.
@@ -195,7 +195,7 @@ Definition pkt6m : packet :=
      pkt_fibkey := fun _ => []; pkt_numgen := fun _ => []; pkt_osf := [];
      pkt_tunnel := fun _ => []; pkt_symhash := fun _ _ => [];
      pkt_xfrm := fun _ _ _ => []; pkt_ctdir := fun _ _ => [];
-     pkt_inner := fun _ _ _ _ => []; pkt_have_l2 := true; pkt_have_l4 := false; pkt_fragoff := 0; pkt_flow := []; pkt_untracked := false; pkt_ctdir_orig := true |}.
+     pkt_inner := fun _ _ _ _ => []; pkt_have_l2 := true; pkt_have_l4 := false; pkt_fragoff := 0; pkt_flow := []; pkt_untracked := false; pkt_ctdir_orig := true; pkt_ct_present := true |}.
 
 (* THE FIX: an ip6 masquerade rewrites the whole 16-byte IPv6 source to the exit
    interface's IPv6 address [if6] (= ipv6_dev_get_saddr), reading back via
