proof/theories/Red_Notrack.v
@@ -76,7 +76,7 @@ Definition pkt_new : packet :=
      pkt_osf := []; pkt_tunnel := fun _ => []; pkt_symhash := fun _ _ => [];
      pkt_xfrm := fun _ _ _ => []; pkt_ctdir := fun _ _ => [];
      pkt_inner := fun _ _ _ _ => []; pkt_have_l2 := true; pkt_have_l4 := false; pkt_fragoff := 0;
-     pkt_flow := [7;7]; pkt_untracked := false; pkt_ctdir_orig := true |}.
+     pkt_flow := [7;7]; pkt_untracked := false; pkt_ctdir_orig := true; pkt_ct_present := true |}.
 
 (* The notrack write threads into rule 2: do_load (LCt CKstate) of the threaded
    packet returns the untracked constant. *)
