proof/theories/Red_NumgenProbe.v
@@ -44,7 +44,7 @@ Definition mkpkt (e : env) (flow : data) : packet :=
      pkt_osf := []; pkt_tunnel := fun _ => []; pkt_symhash := fun _ _ => [];
      pkt_xfrm := fun _ _ _ => []; pkt_ctdir := fun _ _ => [];
      pkt_inner := fun _ _ _ _ => []; pkt_have_l2 := true; pkt_have_l4 := false; pkt_fragoff := 0;
-     pkt_flow := flow; pkt_untracked := false; pkt_ctdir_orig := true |}.
+     pkt_flow := flow; pkt_untracked := false; pkt_ctdir_orig := true; pkt_ct_present := true |}.
 
 (* A one-rule VM program that LOADS `numgen inc mod 2` into reg 1 (the value a
    `numgen ... vmap/map {...}` would dispatch on), then is verdict-neutral
