proof/theories/Tcpflag.v
@@ -52,7 +52,7 @@ Definition pkt_tcpflags (fl : nat) : packet :=
      pkt_fibkey := fun _ => []; pkt_numgen := fun _ => []; pkt_osf := [];
      pkt_tunnel := fun _ => []; pkt_symhash := fun _ _ => [];
      pkt_xfrm := fun _ _ _ => []; pkt_ctdir := fun _ _ => [];
-     pkt_inner := fun _ _ _ _ => []; pkt_have_l2 := true; pkt_have_l4 := true; pkt_fragoff := 0; pkt_flow := []; pkt_untracked := false; pkt_ctdir_orig := true |}.
+     pkt_inner := fun _ _ _ _ => []; pkt_have_l2 := true; pkt_have_l4 := true; pkt_fragoff := 0; pkt_flow := []; pkt_untracked := false; pkt_ctdir_orig := true; pkt_ct_present := true |}.
 
 (* fin=0x01 syn=0x02 rst=0x04 psh=0x08 ack=0x10 urg=0x20 ecn=0x40 cwr=0x80 *)
 
